generic substitution among other things

theories/Harmony.v
@@ -76,7 +76,7 @@ Qed.
 
 Definition try_fnd (d : env) (p : ptcp) := if d.[? p] is Some e then e else EEnd.
 
-Definition map_subst (i : nat) (d : env) g := [fmap x : (domf d) => subst_e i (try_fnd d (val x)) (project g (val x))]. 
+Definition map_subst (i : nat) (d : env) g := [fmap x : (domf d) => (try_fnd d (val x))[s (project g (val x))//i]]. 
 
 
 (*Lemma ptcps_subsitution_aux : forall g0 g1 i, ptcps_of_g g0 `<=` ptcps_of_g (substitution i g0 g1).
@@ -123,109 +123,328 @@ Qed.*)
 
 
 
-Lemma projmap_subst : forall g0  g i S, lpreds [::bound] g -> projmap S (substitution i g0 g) = map_subst i (projmap S g0) g.
+Lemma projmap_subst : forall g0  g i S, lpreds [::bound] g -> projmap S (g0[s g//i]) = map_subst i (projmap S g0) g.
 Proof.
 intros. rewrite /projmap /map_subst. apply/fmapP=>k. rewrite !mapf_if. 
-rewrite (@mapf_if _ _ _ (fun x =>  subst_e i (try_fnd ([fmap p => project g0 (val p)]) (x)) (project g (x)))) /=.
+rewrite (@mapf_if _ _ _ (fun x =>  (try_fnd ([fmap p => project g0 (val p)]) (x))[s (project g (x))//i])) /=.
 rifliad. f_equal. rewrite project_subst. rewrite /try_fnd. rewrite mapf_if H0. done. done. 
 Qed.
 
-Lemma ueqe_subst : forall e0 e1 e' n, (lpreds [::bounde]) e0 -> (lpreds [::bounde]) e1 -> e0 =f= e1 ->  e0[e e'//n] =f= e1[e e'//n].
-Proof. pcofix CIH.  intros. punfold H2. ich H2;simpl;auto.  ich H.
-pfold. constructor. right.  apply : CIH. cc. cc. nth_lpreds 0 H0. rewrite /bounde. by simpl. cc.  nth_lpreds 0 H1. rewrite  /bounde. simpl. eauto. done.
-pfold. constructor. by rewrite !size_map.
-have : (zip (map (fun e0' => (e0')[e e' // n]) gs)  (map (fun e0' => (e0')[e e' // n]) gs')) = map (fun p => (p.1[e e'//n ],p.2[e e'//n])) (zip gs gs'). clear H1 CIH H H0 H3. elim : gs gs'.  destruct gs'. done. by simpl.  destruct gs'. done.
-simpl.  f_equal. apply H. move=>->. induction H3. constructor. rewrite /=. constructor. simpl. right. apply : CIH. cc. ich H0.
-auto. 
-rifliad. pfold. constructor. ich H. rewrite (eqP H0). right.
- rewrite -(@subst_e_nop (g[e ERec n g // n]) e' n). apply : CIH. rewrite -(eqP H0). done.
-Search _ (efv (subst_e _ _ _)).  rewrite Substitutions.efv_subst. by rewrite /= !inE.
-pfold. constructor. right. apply : CIH.
-move : 
-rewrite map_zip.
-right. apply : CIH. move => e0 e1 e' n.
 
-Instance traverse_project_pred_unf : forall g0 g1 i, {goal lpreds rec_pred g0} -> {goal lpreds ([::bound;project_pred]) g1} ->  {goal project_pred (substitution i g0 g1)}.
-Proof. intros. destruct H,H0. constructor.
-elim : g0 g1 i H H0;intros;rewrite /=; simpl in *;try done. 
-- rifliad. cc.
-- cc.  
-- rifliad. cc. cc. apply H;cc.
--  cc; apply H; cc. 
-- have : (project_pred (GBranch a l)) by cc. rewrite /= !big_map. intros. rewrite !all_map. apply/andP.  split. apply/allP=> x' Hin. 
-  simpl. rewrite /projmap. apply/allP=>p. rewrite !inE. intros. apply/ueqeP.
-  erewrite nth_map. rewrite !project_subst. 
-Admitted. 
-(*apply/eqP/fmapP=>k. rewrite !mapf_if. case_if. f_equal.
-  move : Hin. move/nthP=>HH'. specialize HH' with GEnd. destruct HH'. rewrite -H4. erewrite nth_map. 
-  rewrite !project_subst. f_equal. apply :  project_predP_aux. cc. 
-  move : H2. rewrite !inE. move/orP=>[]. rewrite /fresh. destruct ( atom_fresh_for_list ([fset ptcp_from a; ptcp_to a] `|` \bigcup_(j <- l) substitution i j g1)) eqn:Heqn. 
-rewrite Heqn. move/eqP=>->. clear Heqn.
-  move : n. move/negP. rewrite !inE. move/andP=>[]. 
-done. move/andP=>[].  done. done. cc. cc. cc. done.  apply/allP=>k Hin.  simpl. apply H.  done. cc. cc. 
+
+(*Lemma subst_diff : forall e0 e1 e2 k1 k2, k1 <> k2 -> e0[e e1//k1][e e2//k2] = e0[e e2//k2][e e1//k1].
+Proof. Admitted.*)
+
+
+(*Lemma in_subst : forall e e1 n, n \in fv e[s e1//n] = (n \in fv e) && (n \in fv e1).
+Proof. elim;intros;rewrite /= ?inE.
+- rifliad. rewrite eq_sym H /=. done. rewrite /= !inE eq_sym H /=. done. done.
+- rifliad. rewrite !inE neg_sym H0 /=. done. rewrite /= !inE H neg_sym H0 /=. done. rewrite H. done.
+- rewrite !big_map. induction l. rewrite !big_nil !inE. done. rewrite !big_cons !inE. rewrite H. rewrite IHl. destruct (n \in efv a) eqn:Heqn;rewrite Heqn /=.  
+  destruct (n \in efv e1) eqn:Heqn2;rewrite Heqn2 /=. done. lia. done. intros. apply H. auto. auto. 
 Qed.*)
 
 
-
-Instance step_action : forall g l g', {goal step g l g'} -> {goal lpreds [::apred;spred] g} -> {goal apred g'}.  
-Proof.
-move => g l g' [] H [] H0. constructor. elim : H H0; rewrite /=;split_and;cc.
-apply H0. cc.
-apply H0. cc.
-Qed.
-
-Instance step_size : forall g l g',{goal step g l g'} -> {goal lpreds [::apred;spred] g} -> {goal spred g'}.  
-Proof.
-move => g l g' [] H [] H0. constructor.  elim : H H0; rewrite /=;intros;split_and;cc.
-apply H0. cc. rewrite -H.  cc. apply H0. cc. 
-Qed.
+(*Lemma double_subst : forall e0 e1 e2 k1 , e0[e e1//k1][e e2//k1] = e0[e e1//k1].
+Proof. Admitted.*)
 
 
-Instance linear_sgmsg : forall a u g0, {hint Linear (GMsg a u g0)} -> {goal Linear g0}.
+Fixpoint same_vars (e : endpoint ) :=
+match e with 
+| EBranch d c l => all (fun e' => fv (nth EEnd l 0) == fv e') l && (all same_vars l)
+| EMsg _ _ _ e0 => same_vars e0
+| ERec _ e0 => same_vars e0
+| _ => true 
+end.
+
+Fixpoint same_varsg (e : gType ) :=
+match e with 
+| GBranch c l => all (fun e' => fv (nth GEnd l 0) == fv e') l && (all same_varsg l)
+| GMsg _ _ e0 => same_varsg e0
+| GRec _ e0 => same_varsg e0
+| _ => true 
+end.
+
+
+Lemma ueqe_fv : forall e0 e1, e0 =f= e1 -> fv e0 = fv e1. 
+Proof. Admitted.
+
+
+Lemma fv_eq : forall g p, lpreds rec_pred g  -> fv g = fv (project g p). Admitted.
+
+Lemma ppred_same_vars : forall g p, lpreds rec_pred g ->  same_vars (project g p).
 Proof. 
-move => a u g0. apply chint_imp. rewrite /Linear /=.  intros. move : (H (a::aa_p) a0 aa a1). rewrite cat_cons /=. 
-  destruct ( aa_p ++ a0 :: rcons aa a1) eqn:Heqn. case : aa_p H0 Heqn.  done. done.
-  intros. have : Tr ((a::aa_p ++ (a0::aa) ++ [::a1])) (GMsg a u g0). auto.  move/H2 => H3.  move : (H3 H1). 
-  move => [] mi [] mo. intros. auto. 
+elim;rewrite//=;rs;intros. rifliad;simpl;auto. all: try apply H; cc. rifliad;simpl;auto. all : try apply H; cc.
+rifliad. simpl. split_and. apply/allP=>e'. intros. move : H2. move/mapP=>[]. intros. subst.  erewrite nth_map.  
+nth_lpreds 2 H0. simpl. move => HH. apply/eqP/ueqe_fv/ueqeP. split_and. cc. 
+rewrite all_map. apply/allP. intro.  intros. simpl. apply H. done. cc. simpl. 
+split_and. 
+apply/allP=>e'. intros. move : H3. move/mapP=>[]. intros. subst.  erewrite nth_map.  
+nth_lpreds 2 H0. simpl. move => HH. apply/eqP/ueqe_fv/ueqeP. split_and. cc. 
+rewrite all_map. apply/allP. intro.  intros. simpl. apply H. done. cc. 
+rewrite match_n. apply H. cc. cc. 
+Grab Existential Variables. all: repeat constructor.
 Qed.
 
-Instance linear_branch_aux : forall a gs, {hint Linear (GBranch a gs)} -> {goal Forall Linear gs}.  
+Lemma ppred_same_varsg : forall g, lpreds rec_pred g -> same_varsg g.
+Proof.  
+elim;rewrite /=;rs;intros;try done. apply H. cc. apply H.  cc.
+split_and. apply/allP=>e' Hin. erewrite !fv_eq. apply/eqP. apply/ueqe_fv. apply/ueqeP. nth_lpreds 2 H0. simpl. split_and.
+cc. cc. apply/allP=>x. intros. apply H. done. cc. 
+Grab Existential Variables. all : repeat constructor.
+Qed.
+
+
+Lemma subst_distr : forall e e' e2 n n0, lpreds [::bound] e' ->  n<> n0 ->  fv e2 `<=` fv e ->  same_vars e -> e[s e' // n][s e2[s e' // n] // n0] = e[s e2//n0][s e' // n].  
+Proof. 
+elim.
+- intros. simpl. rs. rifliad. by rewrite -(eqP H3)  -(eqP H4)in H0.  simpl. rs. rifliad. rewrite subst_nop.  done. nth_lpreds 0 H.  move/eqP->. by rewrite !inE.  
+  rs. rewrite /= H4. done. rs. by rewrite /= H3 H4.
+- intros. done. 
+- intros. simpl. rs. rifliad. rs. by rewrite /= H5 H4. 
+  rs. rewrite /= H5 H4.  f_equal. f_equal. rewrite (eqP H4) in H2. rewrite subst_nop. done. apply/negP=>HH.  move : (fsubset_in H2 HH). rewrite /= !inE.  split_and. 
+  rs. rewrite (eqP H5) /= eqxx. rewrite -(eqP H5) H4. done. rs. rewrite /= H5 H4 /=.  f_equal.  rewrite H. done. cc. done. rs_in H2.  simpl in H2. apply/fsubsetP=>k. intros. move : (fsubset_in H2 H6). rewrite !inE. split_and. simpl in H3. done.
+- intros. simpl. rs. f_equal. apply H. cc. done. done. done.  
+- intros. simpl. rs. f_equal. rewrite -!map_comp. apply/eq_in_map=>l'. intros. simpl. apply H. done. cc. done. simpl in H2. apply/fsubsetP=>p. intros. move : (fsubset_in H2 H5).  rs.
+  rewrite big_map. rewrite big_exists.  move/hasP=>[]x. intros. simpl in H3. move : p0. move/nthP=>Hnth. specialize Hnth with EEnd. destruct Hnth.
+  suff : p \in fv (nth EEnd l 0). split_and. move : (allP H8 _ H4). move/eqP.   move=><-. done. rewrite -H7 in q. have : nth EEnd l x0 \in l.  cc. intros.
+  split_and.  move :(allP H8 _ x1).  move/eqP. move=>->. done. simpl in H3. split_and. apply (allP H6). done. 
+Qed.
+
+(*Lemma double_inner_subst: forall e e' e2 n n0, lpreds [::bound] e' ->  n<> n0 ->  efv e2 `<=` efv e ->  same_vars e -> e[e e2[e e' // n] // n0][e e' // n] = e[e e2//n0][e e' // n].  
+Proof. 
+elim.
+- intros. simpl. rifliad. rewrite double_subst. done. 
+- intros. done. 
+- intros. simpl. rifliad. simpl. rifliad. simpl in H2. f_equal. f_equal. rewrite (eqP H5) in H3. rewrite subst_nop. done. apply/negP=>HH.  move : (fsubset_in H2 HH). rewrite !inE.  rewrite (eqP H5) eqxx. done.  f_equal.  rewrite H. done. cc. done. simpl in H2. apply/fsubsetP=>k. intros. move : (fsubset_in H2 H6). rewrite !inE. split_and. 
+- intros. simpl. f_equal. simpl in H3. done. 
+- intros. simpl. f_equal. apply : H. cc. done. simpl in H2.  done. simpl in H3. done.
+- intros. simpl. f_equal. rewrite -!map_comp. apply/eq_in_map=>l'. intros. simpl. apply H. done. cc. done. simpl in H2. apply/fsubsetP=>p. intros. move : (fsubset_in H2 H5). 
+  rewrite big_map. rewrite foldr_exists.  move/hasP=>[]x. intros. simpl in H3. move : p0. move/nthP=>Hnth. specialize Hnth with EEnd. destruct Hnth.
+  suff : p \in efv (nth EEnd l 0). split_and. move : (allP H8 _ H4). move/eqP.   move=><-. done. rewrite -H7 in q. have : nth EEnd l x0 \in l.  cc. intros.
+  split_and.  move :(allP H8 _ x1).  move/eqP. move=>->. done. simpl in H3. split_and. apply (allP H6). done. 
+Qed.*)
+
+
+(*Lemma ueqe_subst : forall e0 e1 e' n, (lpreds [::bound])e' ->  e0 =f= e1 ->  e0[e e'//n] =f= e1[e e'//n].
+Proof.  
+elim.
+3 : {  simpl.  intros. rifliad. pfold. constructor. left. rewrite (eqP H2).
+- intros. simpl. rifliad. punfold H0. inversion H0. subst. simpl. rewrite H1. done. subst. simpl. rewrite eq_sym.  H1. 
+pfold. constructor. right.  apply : CIH. cc. cc. 
+pfold. constructor. by rewrite !size_map.
+have : (zip (map (fun e0' => (e0')[e e' // n]) gs)  (map (fun e0' => (e0')[e e' // n]) gs')) = map (fun p => (p.1[e e'//n ],p.2[e e'//n])) (zip gs gs'). clear H2 CIH H H0. elim : gs gs'.  destruct gs'. done. by simpl.  destruct gs'. done.
+simpl.  f_equal. apply H. move=>->. move : H2. move/forallzipP=>HH. apply/Forall_forall. simpl in HH. intros. right. 
+move : H1. move/nthP=>HH'. specialize HH' with (EEnd,EEnd). destruct HH'. rewrite -H2. erewrite nth_map. simpl. apply : CIH. cc.
+erewrite nth_zip. simpl. move : H1.  rewrite size_map size_zip minnE H nat_fact. intros. 
+(*rewrite -H in H1.  cc.
+ cc. erewrite nth_zip.  simpl. move : H2.  rewrite size_map size_zip minnE H nat_fact. intros. cc. done.
+rewrite nth_zip /=. *) suff : upaco2 Unravele bot2 (nth EEnd gs x0) (nth EEnd gs' x0). case. eauto. done. apply : HH. done. rewrite H. done. done.
+move : H1. by rewrite size_map size_zip minnE H nat_fact. 
+rifliad. 
+pfold. constructor. ich H. rewrite (eqP H1). right. 
+ rewrite -(@subst_nop (g[e ERec n g // n]) e' n). apply : CIH. cc. rewrite -(eqP H1). done. 
+rewrite in_subst negb_and. apply/orP. right. by rewrite /= !inE. 
+ich H. pfold. constructor.  right. have : ERec n0 g[e e' // n] = (ERec n0 g)[e e' //n].  rewrite /= H1. done. move=>->. rewrite subst_distr.  
+apply : CIH. cc. done.
+rifliad.*)
+
+Ltac kb d := let Heqn := fresh "Heqn" in destruct d eqn:Heqn;rewrite ?Heqn //=. 
+
+(*TODO*)
+(*Lemma ptcp_subst : forall (A : eqType) (B : choiceType)  x p g1 i (F : A -> {fset B}) , (p \in F (x)[g g1 // i]) = (p \in F x) || ((i \in fv x) && (p \in F g1)).
 Proof.
-move => a gs. apply chint_imp. intros. apply/List.Forall_forall. intros. rewrite /Linear. intros. unfold Linear in H. have : Tr (a::aa_p ++ a0::aa ++ ([::a1])) (GBranch a gs). move : H0.  move/In_in. move/nthP=>Hnth. specialize Hnth with GEnd. destruct Hnth. rewrite -H3 in H1. apply : TRBranch. eauto. apply : H1. 
-intros. apply : H. rewrite -cat_cons in x0. apply : x0. done. 
-Qed.
+elim;rewrite /=;intros.
+- rifliad. by rewrite !inE (eqP H) eqxx /=. by rewrite !inE eq_sym H. by rewrite !inE. 
+- rifliad. rewrite /= !inE (eqP H0) eqxx /=. lia. rewrite /= !inE. rewrite neg_sym. rewrite (negbT H0) /= H. done.
+  rewrite !inE H. by rewrite orbA.  
+- rewrite !big_map. rewrite !inE. kb (p == ptcp_from a). kb (p == ptcp_to a). 
+  clear Heqn Heqn0. induction l. rewrite !big_nil !inE. lia. 
+  rewrite !big_cons !inE H //=. rewrite IHl. rewrite orbA. kb (p \in ptcps_of_g a0).  kb (i \in fv a0). kb (p \in ptcps_of_g g1). lia. 
+  by rewrite andbC /= orbC /=.  intros. apply H. auto. 
+Qed.*)
 
-Instance linear_branch : forall a gs n, {hint Linear (GBranch a gs)} -> {goal n < size gs} -> {goal Linear (nth GEnd gs n)}.
-Proof. intros. destruct H,H0.  apply Build_CHint in H. apply linear_branch_aux in H. destruct H. move : H. move/Forall_forall. intros. constructor. eauto. Qed.
 
-
-Instance linear_unf : forall g n, {hint Linear (GRec n g)} -> {goal Linear g[g GRec n g//n]}.
-Proof. move => g n. apply chint_imp.
-intros.  unfold Linear in *. intros. apply : H. constructor. eauto. done. 
-Qed.
-
-Lemma step_tr : forall g vn g', step g vn g' -> lpreds [::spred] g ->  exists s, Tr (s ++ [::vn.1]) g /\ Forall (fun a => (ptcp_to a) \notin vn.1) s.
+(*Lemma ptcp_subst : forall x p g1 i, (p \in ptcps_of_g (x)[s g1 // i]) = (p \in ptcps_of_g x) || ((i \in fv x) && (p \in ptcps_of_g g1)).
 Proof.
-move => g vn g'. elim.
-- intros. exists nil. rewrite /=. auto.
-- intros. exists nil. rewrite /=. split;auto.  apply TRBranch with (n:=n)(d:=GEnd). done. done.
-- intros.  simpl in H2. destruct H0. cc. destruct H0. exists (a::x). rewrite /=. auto. 
-- intros. move : H1. move/Forall_forall=>Hall. specialize Hall with (nth (GEnd,GEnd) (zip gs gs') 0).
-  rewrite nth_zip in Hall.  simpl in Hall. have : exists s : seq action, Tr (s ++ [:: l.1]) (nth GEnd gs 0) /\ Forall (fun a : action => ptcp_to a \notin l.1) s. apply Hall.  rewrite -nth_zip. apply/mem_nth. rewrite size_zip minnE H. 
-  have :  size gs' - (size gs' - size gs') = size gs' by lia. move=>->. simpl in H3. rewrite -H. cc. lia. cc. intros. destruct x,H1. exists (a::x). simpl. split;auto.  apply TRBranch with (n:=0)(d:=GEnd).  cc. done. done. 
-- intros. destruct H0.  cc. destruct H0. exists x. auto. 
+elim;rewrite /=;intros.
+- rifliad. by rewrite !inE (eqP H) eqxx /=. by rewrite !inE eq_sym H. by rewrite !inE. 
+- rifliad. rewrite /= !inE (eqP H0) eqxx /=. lia. rewrite /= !inE. rewrite neg_sym. rewrite (negbT H0) /= H. done.
+  rewrite !inE H. by rewrite orbA.  
+- rewrite !big_map. rewrite !inE. kb (p == ptcp_from a). kb (p == ptcp_to a). 
+  clear Heqn Heqn0. induction l. rewrite !big_nil !inE. lia. 
+  rewrite !big_cons !inE H //=. rewrite IHl. rewrite orbA. kb (p \in ptcps_of_g a0).  kb (i \in fv a0). kb (p \in ptcps_of_g g1). lia. 
+  by rewrite andbC /= orbC /=.  intros. apply H. auto. 
+Qed. *)
+
+
+(*Lemma big_ptcp_subst : forall l p g1 i, (p \in \bigcup_(j <- l) ptcps (j)[s g1 // i]) = (p \in \bigcup_(j <- l)  ptcps j) || ((i \in \bigcup_(j <- l) fv j) && (p \in ptcps g1)).
+Proof.
+elim;intros;rewrite /= ?big_nil ?big_cons !inE. lia. rewrite H !ptcp_subst orbA. kb (p \in ptcps a). kb (i \in fv a).  
+kb (p \in ptcps g1). lia. kb ((p \in \bigcup_(j <- l) j)). kb ( (p \in \bigcup_(j <- l) g1)). rewrite andbC /=. done. lia. 
+Qed.*)
+
+Lemma big_ptcp_subst_if : forall l g1 i, (\bigcup_(j <- l) ptcps (j)[s g1 // i]) = 
+                                                      if i \in \bigcup_(j <- l) fv j
+                                                          then \bigcup_(j <- l)  ptcps j `|` (ptcps g1) 
+                                                          else \bigcup_(j <- l) ptcps j.
+Proof.
+elim;intros;rewrite /= ?big_nil ?big_cons !inE. done. rewrite H !ptcps_subst. case_if; rewrite H0 /=.  rifliad. fsetPtac. 
+fsetPtac. case_if. fsetPtac. fsetPtac.
 Qed.
 
-(*Linear should be included in *)
+(*Lemma same_vars_subst : forall e0 e1 n, same_vars e0 -> same_vars e1  -> same_vars e0[s e1//n].
+Proof. elim;rewrite /=;rs;intros.  rifliad. done. rifliad. simpl. rs. auto. auto.
+split_and. rewrite all_map. apply/allP=>g' Hin. simpl. erewrite nth_map. rewrite !fv_subst. apply/eqP. f_equal. 
+by apply/eqP/(allP H2). Admitted.*)
+(*Lemma ueqe_subst : forall e0 e1 e' n, same_vars e0 -> same_vars e1 -> bound e' ->  e0 =f= e1 ->  e0[s e'//n] =f= e1[s e'//n].
+Proof. 
+pcofix CIH.  intros. punfold H3. ich H3;simpl;auto.  ich H.
+pfold. constructor. right.  apply : CIH. cc. cc. cc. done.
+pfold. constructor. by rewrite !size_map.
+have : (zip (map (fun e0' => (e0')[s e' // n]) gs)  (map (fun e0' => (e0')[s e' // n]) gs')) = map (fun p => (p.1[s e'//n ],p.2[s e'//n])) (zip gs gs'). clear H2 CIH H H0 H1 H4. elim : gs gs'.  destruct gs'. done. by simpl.  destruct gs'. done.
+simpl.  f_equal. apply H. move=>->. move : H4. move/forallzipP=>HH. apply/Forall_forall. simpl in HH. intros. right. 
+move : H3. move/nthP=>HH'. specialize HH' with (EEnd,EEnd). destruct HH'. rewrite -H4. erewrite nth_map. simpl.
+erewrite nth_zip. simpl. move : H3.  rewrite size_map size_zip minnE H nat_fact. intros. simpl in H0. split_and.
+apply : CIH. 
+apply (allP H6). rewrite -H in H3.  cc. simpl in H1. split_and. apply (allP H7).  cc. done. 
+(*rewrite -H in H1.  cc.
+ cc. erewrite nth_zip.  simpl. move : H2.  rewrite size_map size_zip minnE H nat_fact. intros. cc. done.
+rewrite nth_zip /=. *) suff : upaco2 Unravele bot2 (nth EEnd gs x0) (nth EEnd gs' x0). case. eauto. done. apply : HH. done. rewrite H. done. done.
+move : H3. by rewrite size_map size_zip minnE H nat_fact. rs. 
+rifliad. 
+pfold. constructor. ich H. rewrite (eqP H3). right. 
+rewrite -(@subst_nop _ (g[s ERec n g // n]) e' n). apply : CIH. cc. Admitted. *)
+(*rewrite -(eqP H1). done. 
+rewrite in_subst negb_and. apply/orP. right. by rewrite /= !inE. 
+ich H. pfold. constructor.  right.  have : ERec n0 g[e e' // n] = (ERec n0 g)[e e' //n].  rewrite /= H1. done. move=>->. rewrite subst_distr. 
+apply : CIH. cc. rewrite -H2.  done. cc. lia. simpl. apply/fsubsetP=>k. rewrite !inE. split_and. done. rewrite !inE. done.
+rifliad.*)
+
+
+
+(*pfold. constructor. ich H. right. rewrite subst_diff. apply : CIH. cc. move : H0. unlock lpreds. rewrite /=. nth_lpreds 0 H1. rewrite /bound. split_and.
+rewrite Substitutions.efv_subst. simpl in H. done. rewrite /ebound. simpl. rewrite Substitutions.efv_subst.
+simpl in H.  rewrite -(eqP H). apply/eqP/fsetP=>k. rewrite !inE. destruct (eqVneq k n0);rewrite /=. done.
+destruct (eqVneq k n);rewrite /=. subst.
+ Check (@subst_nop (g[e ERec n0 g // n]) e' n0). apply : CIH. rewrite -(eqP H2). cc. cc.  rewrite -(eqP H2). done.
+ rewrite Substitutions.efv_subst. by rewrite /= !inE. cc. rewrite -(eqP H2). cc.
+
+pfold. constructor. right. apply : CIH.
+move : 
+rewrite map_zip.
+right. apply : CIH. move => e0 e1 e' n.*)
+
+
+
+(*Add constraint that g1 participants is subset of g0's participants*)
+
+Lemma fresh_for : forall S S', S' `<=` S -> fresh S \notin S'.
+Proof.  intros. rewrite /fresh. destruct (atom_fresh_for_list S). apply/negP=>HH. apply : n. by apply (fsubset_in H). Qed.
+
+
+
+(*Lemma project_pred_ptcps : forall a gs i p, lpreds (rec_pred) (GBranch a gs) -> p \in (fv (GBranch a gs)) -> i < size gs -> p \in  fv (nth GEnd gs i).
+Proof. intros.  destruct (atom_fresh_for_list ([::ptcp_from a;ptcp_to a])). nth_lpreds 0 H=>HH. move : HH. 
+rewrite /rec_pred.
+rewrite !(@fv_project_eq _ x).  move : n. move/negP. rewrite !inE. rewrite /=. split_and. move : HH. rewrite (negbTE H1) (negbTE H3). 
+Qed.
+
+ Lemma project_pred_ptcps2 : forall a gs i p, lpreds rec_pred (GBranch a gs) -> i < size gs ->  (p \in  fv (nth GEnd gs i)) ->  (p \in fv (GBranch a gs)).
+Proof. intros.  rewrite /= big_map.  rewrite foldr_exists. apply/hasP.  exists (nth GEnd gs i). cc. done. 
+Qed.
+
+
+Lemma project_pred_ptcps_set : forall a gs i, lpreds rec_pred (GBranch a gs) -> i < size gs -> fv (GBranch a gs) = fv (nth GEnd gs i).
+Proof.
+intros. apply/fsetP. move => x.  destruct ((x \in fv (nth GEnd gs i))) eqn:Heqn.
+erewrite project_pred_ptcps2. done. cc. eauto. done. destruct ( (x \in fv (GBranch a gs)))eqn:Heqn2. erewrite project_pred_ptcps in Heqn. done. have : ipred x (GBranch a gs).  cc. intros.  cc. cc. cc. 
+Qed.*)
+
+Lemma traverse_project_pred_unf : forall g0 g1 i, ppred g0 && ppred g1 -> ppred g0[s g1// i].
+Proof. 
+intros. destruct (i \notin fv g0) eqn:Heqn. rewrite subst_nop //=. split_and. 
+elim : g0 g1 i Heqn H;intros;rewrite /=. 
+- move : Heqn. rewrite /= !inE. move/negbT. rewrite !inE. rewrite eq_sym.  rs. move=>->. done. done. 
+- move : Heqn. rs.  rewrite /= !inE. move/orP/orP. rewrite !inE. split_and. have: n == i = false by lia. move=>->. 
+  simpl. apply H. by rewrite H2. 
+- split_and. 
+- split_and. apply H. done. split_and.
+- rewrite /= !big_map !all_map big_ptcp_subst_if. apply/andP.  split. rifliad. 
+ * apply/allP=> x' Hin. simpl. apply/allP=>p. rewrite !inE. intros. split_and. 
+ * rs. rs_in Heqn. split_and.  rewrite /= big_map H1 in Heqn. done. 
+ * apply/allP=>g'. intros. simpl. apply H. done. suff : i \in fv g'. by  move=>->. 
+   have : i \in fv (GBranch a l). lia. split_and. move : (ppred_same_varsg H2). simpl. split_and.  rs_in x. rewrite /= big_map big_exists in x. destruct (hasP x). rewrite -(eqP (allP H0 _ H5)) in H6. rewrite -(eqP (allP H0 _ H1)). done. split_and. simpl in H2. split_and. by apply (allP H4).
+Qed.
+
+(*Lemma traverse_project_pred_unf : forall g0 g1 i, lpreds rec_pred g0 -> lpreds ([::bound;project_pred]) g1 -> g1 `<=` g0 -> project_pred (substitution i g0 g1).
+Proof. 
+elim;intros;rewrite /=; simpl in *;try done. 
+- rifliad. cc.
+- rifliad. cc. simpl. apply H. cc. cc. done.
+- apply H. cc. cc. admit.
+- have : (project_pred (GBranch a l)) by cc. rewrite /= !big_map. intros. rewrite !all_map. apply/andP.  split. 
+ * apply/allP=> x' Hin. simpl. apply/allP=>p. rewrite !inE. intros. apply/ueqeP.
+   erewrite nth_map. rewrite !project_subst. apply ueqe_subst. apply ppred_same_vars.  cc. apply ppred_same_vars. cc. cc. 
+   split_and. move : H3.  move/orP=>[]. move/eqP=>->. 
+(*  have :  project (nth GEnd l 0) (fresh (a `|` \bigcup_(j <- l) (j)[s g1 // i])) =  project (nth GEnd l 0) (fresh (a `|` \bigcup_(j <- l) j)).*)
+  erewrite project_tw0.  apply/ueqeP/(allP (allP H4 _ Hin)). rewrite !inE. apply/orP. left. 
+  rewrite big_ptcp_subst_if. rifliad.
+
+   have : (a `|` (\bigcup_(j <- l) j `|` g1)) = a`|`  \bigcup_(j <- l) j.
+  apply/fsetP=>k. rewrite !inE. kb (k == ptcp_from a). kb (k ==ptcp_to a). move : (fsubset_in H2).  move=>Hf. kb (k \in ptcps g1). rewrite orbC /=. apply Hf in Heqn1. by  rewrite !inE Heqn Heqn0 /= big_map in Heqn1. by rewrite orbC /=. 
+  move=>->. done.  cc.
+
+  rewrite /npred. rewrite big_ptcp_subst_if. rifliad. Search _ fresh. rewrite /fresh. destruct (atom_fresh_for_list  (a `|` \bigcup_(j <- l) (j)[s g1 // i]) ) eqn:Heqn. rewrite Heqn.
+  apply/negP=>HH. apply n. move : HH. rewrite !inE. intros. apply/orP. right. rewrite foldr_exists. apply/hasP. exists (nth GEnd l 0). cc.
+  rewrite ptcp_subst HH. done. 
+
+  rewrite /npred. rewrite /fresh. destruct (atom_fresh_for_list  (a `|` \bigcup_(j <- l) j)) eqn:Heqn. rewrite Heqn.
+  apply/negP=>HH. apply n. move : HH. rewrite !inE. intros. apply/orP. right. rewrite foldr_exists. apply/hasP. exists (nth GEnd l 0). cc.
+  done.
+  move=>->. 
+
+  have :  project x'  (fresh (a `|` \bigcup_(j <- l) (j)[s g1 // i])) =  project x' (fresh (a `|` \bigcup_(j <- l) j)). admit.
+  move=>->.
+
+
+  apply/ueqeP. apply/(allP (allP H4 _ Hin)) . by rewrite !inE. 
+  split_and. rewrite (negbTE H7) (negbTE H8) /= in H6. move : H6. rewrite foldr_exists. move/hasP=>[]. intros.
+  apply/ueqeP/(allP (allP H4 _ p0)). rewrite !inE. apply/orP. left. done. cc. cc. cc. right. split_and. eauto. auto. rewrite (negbTE H7) (negbTE H8) /=. 
+  rewrite foldr_exists. apply/hasP. exists x. done. rewrite ptcp_subst in q. destruct (orP q). done. split_and.
+
+
+  split_and. apply/ueqeP. apply/(allP (allP H3 _ Hin)) . rewrite !inE H6 H7 /=. destruct (orP H5). destruct (orP H2). rewrite H8. apply/orP.  right. done. 
+  rewrite H8. apply/orP. right. apply/orP.   left. by rewrite orbC.   rewrite H2. 
+lia.
+
+move : H2. rewrite !inE. move/orP=>[]. move/eqP=>->. move/orP=>[]. rewrite eqxx. . move=>Hall. 
+
+  apply project_tw0. cc. 
+  rewrite /npred. rewrite /fresh. destruct (atom_fresh_for_list  (a `|` \bigcup_(j <- l) (j)[s g1 // i]) ) eqn:Heqn. rewrite Heqn.
+  apply/negP=>HH. apply n. move : HH. rewrite !inE. intros. apply/orP. right. rewrite foldr_exists. apply/hasP. exists (nth GEnd l 0). cc.
+  apply ptcp_in_subst. done. 
+
+  rewrite /npred. rewrite /fresh. destruct (atom_fresh_for_list  (a `|` \bigcup_(j <- l) j)) eqn:Heqn. rewrite Heqn.
+  apply/negP=>HH. apply n. move : HH. rewrite !inE. intros. apply/orP. right. rewrite foldr_exists. apply/hasP. exists (nth GEnd l 0). cc.
+  done.
+  move=>->. 
+
+cc. nth_lpreds n H*)
+
+
+
+
+
+
+
+
 
 Definition linear (g : gType) := true. 
 Lemma linearP : forall g, reflect (Linear g)  (linear g) . 
 Admitted.
 
 
-
-
-(*Lemma In_exists : forall (A : Type) (a : A) l, In a l -> exists (l0 l1 : seq A), l = l0 ++ (a::l).*)
 Lemma ch_diff : forall g a0 aa a1, lpreds [::linear] g -> Tr (a0::(aa++[::a1])) g  -> Forall ( fun a => (ptcp_to a) \notin a1) (a0::aa) ->  Forall (fun a => action_ch a != action_ch a1) (a0::aa).
 Proof.
 intros. apply/List.Forall_forall. intros. 
@@ -244,6 +463,19 @@ have : (a0 :: (x0 ++ (x :: x1)%SEQ)%list ++ [:: a1]) = ((a0 :: x0) ++ x :: x1 ++
   rewrite H2. intros. inversion H1. apply List.Forall_app in H8. destruct H8. inversion H9. apply : no_indep. 
   apply H12.  apply H13.  done.
 Qed.
+
+Lemma step_tr : forall g vn g', step g vn g' -> size_pred g ->  exists s, Tr (s ++ [::vn.1]) g /\ Forall (fun a => (ptcp_to a) \notin vn.1) s.
+Proof.
+move => g vn g'. elim.
+- intros. exists nil. rewrite /=. auto.
+- intros. exists nil. rewrite /=. split;auto.  apply TRBranch with (n:=n)(d:=GEnd). done. done.
+- intros.  simpl in H2. destruct H0. done. destruct H0. exists (a::x). rewrite /=. auto. 
+- intros. move : H1. move/Forall_forall=>Hall. specialize Hall with (nth (GEnd,GEnd) (zip gs gs') 0).
+  rewrite nth_zip in Hall.  simpl in Hall. have : exists s : seq action, Tr (s ++ [:: l.1]) (nth GEnd gs 0) /\ Forall (fun a : action => ptcp_to a \notin l.1) s. apply Hall.  rewrite -nth_zip. apply/mem_nth. rewrite size_zip minnE H. 
+  have :  size gs' - (size gs' - size gs') = size gs' by lia. move=>->. simpl in H3. rewrite -H. split_and. done.  simpl in H3. split_and. apply (allP H4). apply/mem_nth. done.  intros. destruct x,H1. exists (a::x). simpl. split;auto.  apply TRBranch with (n:=0)(d:=GEnd).  simpl in H3. split_and. done. done. 
+- intros. destruct H0.  apply size_pred_subst. done. done.  exists x. split.  destruct H0. constructor. done. destruct H0. done. 
+Qed.
+
 
 Lemma distinct_ch : forall g vn g', step g vn g' -> lpreds [::linear;size_pred] g ->  exists s, Tr (s ++ [::vn.1]) g /\  Forall (fun a =>  (action_ch a) != (action_ch vn.1)) s.
 Proof. intros. edestruct (step_tr). eauto. cc. destruct H1. exists x. split;auto. inversion H2. done. apply : ch_diff. cc. 
@@ -268,7 +500,7 @@ Proof. move => g l g'. elim.
   rifliad.
  * constructor. auto. apply H0.  cc. apply/eqP. rewrite neg_sym.  apply : distinct_ch_msg.  eauto. eauto. cc. 
  * apply : H0. cc. 
-- intros. rewrite /=. move : H2. move/[dup]. move=>H2 Hdup. rewrite !inE in H2. split_and. rewrite eq_sym. rifliad.
+- intros. rewrite /=. move : H2. move/[dup]. move=>H2 Hdup.  rewrite !inE in H2. split_and. rewrite eq_sym. rifliad.
  * constructor. auto. rewrite !size_map. done. apply/Forall_forall. move => x. 
    move/nthP=>HH. specialize HH with (EEnd,EEnd). destruct HH. 
  move : H6.  rewrite size_zip !size_map  H minnE nat_fact. intros. 
@@ -292,9 +524,9 @@ clear H4. rewrite nth_zip in H7. rewrite -H7 /=.
    rewrite nth_zip in Hall. simpl in Hall. apply Hall. rewrite -nth_zip. apply/mem_nth. rewrite size_zip minnE H.
    have : size gs' - (size gs' - size gs') = size gs' by lia. move=>->. simpl in H4. rewrite -H. cc. all : cc. 
 - intros. (*have : lpreds rec_pred (GRec n g0) by cc. clear H3. move=> H3.*) rewrite /=. rifliad. 
- * rewrite !project_subst in H0.  rewrite (eqP H2) /= eqxx H2 in H0. apply H0.  cc. cc. 
- * econstructor. pfold.  econstructor. left. eauto. rewrite /= !project_subst /= in H0. rewrite H2 H3 in H0.   apply H0. cc. cc. 
-- rewrite /= !project_subst /= in H0. rewrite H2 H3 in H0. rewrite subst_nop in H0. apply H0. cc. by rewrite H3. cc. 
+ * rewrite !project_subst in H0.  rewrite (eqP H2) /= H2 in H0. rs_in H0. rewrite eqxx  in H0. apply H0.  cc. cc. apply  traverse_project_pred_unf. split_and. cc. cc. cc.
+ * econstructor. pfold.  econstructor. left. eauto. rewrite /= !project_subst /= in H0. rewrite H2 H3 in H0.   apply H0. cc. cc. apply traverse_project_pred_unf. split_and.  cc. cc. cc.
+- rewrite /= !project_subst /= in H0. rewrite H2 H3 in H0. rewrite !subst_nop in H0. apply : H0. cc. nth_lpreds 0 H1. rewrite /bound. move/eqP=><-. rs. apply/eqP. rewrite mem_fsetD1 //=. erewrite fv_eq. lia. by apply/negbT. erewrite fv_eq. apply/negbT. eauto. cc. 
 Grab Existential Variables. eauto.
 Qed.
 
@@ -323,9 +555,10 @@ clear H4. rewrite nth_zip in H7. rewrite -H7 /=.
  * apply/eqP. rewrite neg_sym. apply : distinct_ch_branch. eauto. eauto. cc.
    move : H1. move/forallzipP=>HH. simpl in HH. apply : HH. done. cc. cc.
 - intros. (*have : lpreds rec_pred (GRec n g0) by cc. clear H3. move=> H3.*) rewrite /=. rifliad. 
- * rewrite !project_subst in H0.  rewrite (eqP H2) /= eqxx H2 in H0. apply H0.  cc. cc. 
- * econstructor. pfold.  econstructor. left. eauto. rewrite /= !project_subst /= in H0. rewrite H2 H3 in H0.   apply H0. cc. cc. 
-- rewrite /= !project_subst /= in H0. rewrite H2 H3 in H0. rewrite subst_nop in H0. apply H0. cc. by rewrite H3. cc. 
+ * rewrite !project_subst in H0.  rs_in H0. rewrite H2 (eqP H2) in H0.  rs_in H0. rewrite eqxx in H0. apply H0.  cc. 
+ * apply traverse_project_pred_unf.  split_and. cc. cc. cc. econstructor. pfold.  econstructor. left. eauto. rewrite /= !project_subst /= in H0. rewrite H2 H3 in H0.   apply H0. cc. apply traverse_project_pred_unf. split_and. cc. cc. cc.
+- rewrite /= !project_subst /= in H0. rewrite H2 H3 in H0. rewrite !subst_nop in H0. apply H0. cc. 
+ nth_lpreds 0 H1. rewrite /bound. move/eqP=><-. rs. apply/eqP. rewrite mem_fsetD1 //=. erewrite fv_eq. lia. by apply/negbT. erewrite fv_eq. apply/negbT. eauto. cc. 
 Grab Existential Variables. eauto.
 Qed.
 
@@ -349,9 +582,9 @@ move => g l g'. elim;intros.
 
   rewrite !match_n. move : H1. move/Forall_forall=>Hfor. specialize Hfor with (nth (GEnd,GEnd) (zip gs gs') 0) p. rewrite nth_zip /= in Hfor. apply Hfor.  rewrite -nth_zip. apply/mem_nth.  rewrite size_zip minnE H nat_fact -H. cc. done. cc. done. done. 
 - simpl.  rifliad. 
-- intros.  apply : ueqe_trans.  2 : { apply : H0. cc. done. } rewrite project_subst. rewrite (eqP H3) /= eqxx H3. auto. cc.
- * apply : ueqe_trans.  2 : { apply : H0. cc. done. } pfold. rewrite project_subst. constructor. left. rewrite /= H3 H4.  auto. cc. 
-   apply : ueqe_trans. 2 : {  apply : H0. cc. done. } rewrite project_subst /=. rewrite H3 H4. rewrite subst_e_nop. auto.
+- intros.  apply : ueqe_trans.  2 : { apply : H0. cc. apply traverse_project_pred_unf.  split_and. cc. cc. done. } rewrite project_subst. rs. rewrite H3  (eqP H3) /=. rs. rewrite eqxx. auto. cc.
+ * apply : ueqe_trans.  2 : { apply : H0. cc. apply traverse_project_pred_unf. split_and. cc. cc. done. } pfold. rewrite project_subst. constructor. left. rewrite /= H3 H4.  auto. cc. 
+   apply : ueqe_trans. 2 : {  apply : H0. cc. apply traverse_project_pred_unf. split_and. cc. cc. done. } rewrite project_subst /=. rewrite H3 H4. rewrite subst_nop. auto.
    apply/negP. by rewrite H4. cc.
 Qed.
 
