theories/Structures.v
@@ -5,7 +5,7 @@ Set Implicit Arguments.
 Unset Strict Implicit.
 Unset Printing Implicit Defensive.
 
-From Dep Require Import Global_Syntax Substitutions Predicates.
+From Dep Require Import Global_Syntax Inductive_Linearity Substitutions Predicates.
 Let inE := Predicates.inE.
 
 
@@ -18,11 +18,7 @@ Ltac norm_eqs := repeat (match goal with
                    | [ H : is_true (?a != ?a_) |- _ ] => rewrite eqxx in H;done 
 
                   end).
-Ltac split_and := intros;repeat (match goal with 
-                   | [ H : is_true (_ && _) |- _ ] => destruct (andP H);clear H
-                   | [ |- is_true (_ && _) ] => apply/andP;split 
 
-                  end);auto.
 
 
 Definition preds (A : eqType) (l : seq (pred A)) : pred A := (foldr predI predT l).
@@ -52,7 +48,7 @@ Instance CGoal_Hint `{H : CHint D} : CGoal D. destruct H. constructor. done. Def
 
 
 
-Lemma notin_big : forall (p : ptcp) gs i, p \notin \bigcup_(j <- gs) (ptcps_of_g j) -> i < size gs -> p \notin ptcps_of_g (nth GEnd gs i).
+Lemma notin_big : forall (p : ptcp) gs i, p \notin \bigcup_(j <- gs) (ptcps j) -> i < size gs -> p \notin ptcps (nth GEnd gs i).
 Proof.
 intros. apply/negP=>HH. apply (negP H). apply/bigfcupP. exists (nth GEnd gs i). rewrite mem_nth //=. apply HH. Qed.
 
@@ -72,8 +68,8 @@ Ltac usl := ul; rewrite /= lock_lpreds.
 
 Ltac apply_typeclasses := to_goal;typeclasses eauto with typeclass_instances.
 Ltac pre_process := unlock lpreds;rewrite /=;split_and.
-Definition notin_pred p g :=  p \notin (ptcps_of_g g).  
-Lemma notin_pred_eq p : notin_pred p =  (fun g => p \notin (ptcps_of_g g)). done. Qed.
+Definition notin_pred p g :=  p \notin (ptcps g).  
+Lemma notin_pred_eq p : notin_pred p =  (fun g => p \notin (ptcps g)). done. Qed.
 
 
 Ltac cc := match goal with 
@@ -110,7 +106,7 @@ Notation ppred := project_pred.
 
 Definition rec_pred := [::apred;spred;ppred]. 
 
-Class CGPred (A : eqType) (p : pred A) := { _ : pred gType }.
+Class CGPred (A : eqType) (p : pred A) := { _ : pred A }.
 
 Instance apred_CGPred : CGPred apred. constructor. constructor. Qed.
 Instance spred_CGPred : CGPred spred. constructor. constructor. Qed.
@@ -147,8 +143,8 @@ Lemma In_l_preds : forall (A : eqType) l (g : A) p, In p l -> lpreds l g ->  p g
 Proof. move=> A. elim. done. simpl. intros. destruct H0. subst.  move : H1. unlock lpreds. simpl. lia. apply H. done. move : H1. unlock lpreds. simpl. lia. 
 Qed.
 
-Instance resolve_to_lpreds  : forall (l : seq (pred gType)) g0 g1 p, CGPred p -> {hint lpreds l g0} -> CFind p l ->  CStructural p g0 g1 -> {goal p g1}.
-Proof. move => l g0 g1 p [] H [] H0 [] H1 [] H2. constructor. apply H2. apply : In_l_preds;eauto. Qed.
+Instance resolve_to_lpreds  : forall (A : eqType ) (l : seq (pred A)) g0 g1 p, CGPred p -> {hint lpreds l g0} -> CFind p l ->  CStructural p g0 g1 -> {goal p g1}.
+Proof. move => A l g0 g1 p [] H [] H0 [] H1 [] H2. constructor. apply H2. apply : In_l_preds;eauto. Qed.
 
 
 Lemma index_lpreds : forall (A :eqType) l (g : A) n, lpreds l g -> (nth (fun _ => true) l n g).
@@ -182,9 +178,9 @@ eapply notin_big in H1. apply : H1. done. Qed.
 Instance Goal_msg_action a v g : {goal (apred (GMsg a v g))} -> {goal ptcp_from a != ptcp_to a}. move=>[] H. constructor. simpl in H. split_and. Qed.
 Instance Goal_branch_action a gs : {goal (apred (GBranch a gs))} -> {goal ptcp_from a != ptcp_to a}. move=>[] H. constructor. simpl in H. split_and. Qed.
 
-Instance traverse_action_pred_unf : forall g0 g1 i, {goal lpreds [::apred] g0} -> {goal lpreds [::apred] g1} -> {goal apred (substitution i g0 g1)}.
+Instance traverse_action_pred_unf : forall g0 g1 i, {goal lpreds [::apred] g0} -> {goal lpreds [::apred] g1} -> {goal apred (g0[s g1//i])}.
 Proof.  intros. destruct H,H0. constructor.
-elim : g0 g1 i H H0 ;intros;rewrite /=;try done. 
+elim : g0 g1 i H H0 ;intros;rewrite /=;rs;try done. 
 - rifliad. cc. 
 - rifliad. cc.  apply H;cc. 
 - split_and; cc. apply : H; cc. 
@@ -194,33 +190,33 @@ Qed.
 (*Instance traverse_action_pred_unfG : forall g0 g1 i, {goal lpreds [::apred] g0} -> {goal lpreds  [::apred] g1} -> {goal lpreds  [::apred]  (substitution i g0 g1)}.
 Proof. intros. constructor. destruct H,H0. apply traverse_action_pred_unf;cc. Qed.
 *)
-Instance traverse_size_pred_unf : forall g0 g1 i, {goal lpreds [::spred] g0} -> {goal lpreds [::spred] g1} -> {goal spred (substitution i g0 g1)}.
-Proof.  intros. constructor.  destruct H ,H0. 
-elim : g0 g1 i H H0;intros;rewrite /=; simpl in *;try done;auto.
-- rifliad. cc. 
-- rifliad. cc. apply H. cc. cc. 
-- apply H. cc. cc. 
-- split_and. rewrite size_map. cc. 
-- rewrite all_map. apply/allP=> ll Hin /=. apply : H;cc. 
+
+Lemma size_pred_subst : forall g0 g1 i, size_pred g0 -> size_pred g1 -> size_pred (g0[s g1//i]).
+Proof.  
+elim;intros;rewrite /=;rs; simpl in *;try done;auto.
+- rifliad. rifliad. simpl.  auto. 
+- rewrite all_map. apply/andP. split. rewrite size_map. split_and. apply/allP=> ll Hin /=. apply H. done. split_and. apply (allP H3). done. done. 
 Qed.
 
-(*Instance traverse_size_pred_unfG : forall g0 g1 i, {goal lpreds [::size_pred] g0} -> {goal lpreds [::size_pred] g1} -> {goal lpreds [::size_pred] (substitution i g0 g1)}.
-Proof. intros. constructor. destruct H,H0.  apply traverse_size_pred_unf;cc. Qed.
-*)
 
-
-Instance bound_CGPred : CGPred bound. repeat constructor. Qed.
-Instance CStructural_bound_msg a u g: CStructural bound (GMsg a u g) g.
-constructor. rewrite /bound /=. done. Qed.
+Instance traverse_size_pred_unf : forall g0 g1 i, {goal lpreds [::spred] g0} -> {goal lpreds [::spred] g1} -> {goal spred (g0[s g1//i])}.
+Proof.  intros.  constructor.  apply size_pred_subst.   destruct H. cc. destruct H0. cc. Qed.
+Print bound.
+Check @bound. Check CGPred.
+Instance bound_CGPred (A : substType) : CGPred (@bound A). repeat constructor. Qed.
+Check CStructural.
+Check bound.
+Instance CStructural_bound_msg  a u g: CStructural (bound)  (GMsg a u g) g.
+constructor. rewrite  /=. done. Qed.
 
 Instance  CGoal_all_boundb a gs : {goal bound (GBranch a gs)} -> {goal all bound gs}. 
-move => [] H. constructor.  unfold bound in H. simpl in H. move : H.  rewrite big_map. rewrite /bound. induction gs. rewrite big_nil. done. rewrite big_cons. rewrite /=. move/eqP=>HH. rewrite IHgs //=. split_and. 
+move => [] H. constructor.  simpl in H. move : H. rewrite /bound.  rs. rewrite big_map. induction gs. rewrite big_nil. done. rewrite big_cons. rewrite /=. move/eqP=>HH. rewrite IHgs //=. split_and. 
 apply/eqP/fsetP=>k. rewrite !inE.
-have :  (k \in fv_g a0 `|` \bigcup_(j <- gs) fv_g j) = (k \in fset0). move : HH. move/fsetP=>HH. rewrite HH. done. 
+have :  (k \in fv a0 `|` \bigcup_(j <- gs) fv j) = (k \in fset0). move : HH. move/fsetP=>HH. rewrite HH. done. 
 rewrite !inE. move/orP/orP. rewrite negb_or. split_and. by apply/negbTE. 
 
 apply/eqP/fsetP=>k. rewrite !inE.
-have :  (k \in fv_g a0 `|` \bigcup_(j <- gs) fv_g j) = (k \in fset0). move : HH. move/fsetP=>HH. rewrite HH. done. 
+have :  (k \in fv a0 `|` \bigcup_(j <- gs) fv j) = (k \in fset0). move : HH. move/fsetP=>HH. rewrite HH. done. 
 rewrite !inE. move/orP/orP. rewrite negb_or. split_and. by apply/negbTE. 
 Qed.
 
@@ -229,50 +225,51 @@ Instance  CStructural_boundb a gs g : {goal g \in gs} ->  CStructural bound (GBr
 Proof. move=>[] H. constructor.  move/Build_CGoal. move/CGoal_all_boundb=>[]. move/allP=>Hall. apply Hall. done. 
 Qed.
 
-Instance bound_unf g n : {goal bound (GRec n g)} -> {goal bound (g[g GRec n g//n])}.
-Proof. move => [].  constructor. move : b.  rewrite /bound. intros. rewrite fv_g_unf /=. by simpl in b. 
-cc. Qed.
+Instance bound_unf g n : {goal bound (GRec n g)} -> {goal bound (g[s GRec n g//n])}.
+Proof. move => [].  constructor. move : b. intros.  rewrite /bound. rewrite fv_subst  /=.  by simpl in b. 
+rs. rs_in b. by apply/eqP. Qed.
 
 
 
-Instance bounde_CGPred : CGPred bounde. repeat constructor. Qed.
-Instance CStructural_bounde_msg d a u g: CStructural bounde (EMsg d a u g) g.
-constructor. rewrite /bounde /=. done. Qed.
+(*Instance bounde_CGPred : CGPred bounde. repeat constructor. Qed.*)
 
-Instance  CGoal_all_boundeb d a gs : {goal bounde (EBranch d a gs)} -> {goal all bounde gs}. 
-move => [] H. constructor.  unfold bounde in H. simpl in H. move : H.  rewrite big_map. rewrite /bounde. induction gs. rewrite big_nil. done. rewrite big_cons. rewrite /=. move/eqP=>HH. rewrite IHgs //=. split_and. 
+
+Instance CStructural_bounde_msg d a u g: CStructural bound (EMsg d a u g) g.
+constructor. rewrite  /=. done. Qed.
+
+Instance  CGoal_all_boundeb d a gs : {goal bound (EBranch d a gs)} -> {goal all bound gs}. 
+move => [] H. constructor.  simpl in H. move : H.  rewrite /bound. rs. rewrite big_map.  induction gs. rewrite big_nil. done. rewrite big_cons. rewrite /=. move/eqP=>HH. rewrite IHgs //=. split_and. 
 apply/eqP/fsetP=>k. rewrite !inE.
-have :  (k \in efv a0 `|` \bigcup_(j <- gs) efv j) = (k \in fset0). move : HH. move/fsetP=>HH. rewrite HH. done. 
+have :  (k \in fv a0 `|` \bigcup_(j <- gs) fv j) = (k \in fset0). move : HH. move/fsetP=>HH. rewrite HH. done. 
 rewrite !inE. move/orP/orP. rewrite negb_or. split_and. by apply/negbTE. 
 
 apply/eqP/fsetP=>k. rewrite !inE.
-have :  (k \in efv a0 `|` \bigcup_(j <- gs) efv j) = (k \in fset0). move : HH. move/fsetP=>HH. rewrite HH. done. 
+have :  (k \in fv a0 `|` \bigcup_(j <- gs) fv j) = (k \in fset0). move : HH. move/fsetP=>HH. rewrite HH. done. 
 rewrite !inE. move/orP/orP. rewrite negb_or. split_and. by apply/negbTE. 
 Qed.
 
 
-Instance  CStructural_boundeb d a gs g : {goal g \in gs} ->  CStructural bounde (EBranch d a gs) g. 
+Instance  CStructural_boundeb d a gs g : {goal g \in gs} ->  CStructural bound (EBranch d a gs) g. 
 Proof. move=>[] H. constructor.  move/Build_CGoal. move/CGoal_all_boundeb=>[]. move/allP=>Hall. apply Hall. done. 
 Qed.
 
-Instance bounde_unf g n : {goal bounde (ERec n g)} -> {goal bounde (g[e ERec n g//n])}.
-Proof. move => [].  constructor. move : b.  rewrite /bounde. intros.  rewrite Substitutions.efv_subst /=. by simpl in b. 
-cc. Qed.
+Instance bounde_unf g n : {goal bound (ERec n g)} -> {goal bound (g[s ERec n g//n])}.
+Proof. move => [].  constructor. move : b.   intros.   rewrite /bound. rewrite fv_subst /=. by simpl in b. 
+rs. rs_in b. by apply/eqP. Qed.
 
-
-Instance goallpreds_cons (p : pred gType) g (l : seq (pred gType)): {goal p g} -> {goal (lpreds l g) } -> {goal lpreds (p::l) g}. move => [] H [] H0. constructor. unlock lpreds. simpl. unlock lpreds in H0.  split_and. Qed.
+Instance goallpreds_cons (A : eqType) (p : pred A) g (l : seq (pred A)): {goal p g} -> {goal (lpreds l g) } -> {goal lpreds (p::l) g}. move => [] H [] H0. constructor. unlock lpreds. simpl. unlock lpreds in H0.  split_and. Qed.
 
 Instance goallpreds_nil (A : eqType) (g : A) : {goal lpreds nil g}. constructor. unlock lpreds. simpl. done. Qed. 
 
-Instance goallpreds_allcons (p : pred gType) gs (l : seq (pred gType)): {goal all p gs} -> {goal all (lpreds l) gs } -> {goal all (lpreds (p::l)) gs}. move => [] H [] H0. constructor. unlock lpreds. simpl. unlock lpreds in H0. rewrite all_predI. split_and. Qed.
+Instance goallpreds_allcons (A : eqType) (p : pred A) gs (l : seq (pred A)): {goal all p gs} -> {goal all (lpreds l) gs } -> {goal all (lpreds (p::l)) gs}. move => [] H [] H0. constructor. unlock lpreds. simpl. unlock lpreds in H0. rewrite all_predI. split_and. Qed.
 
-Lemma lpredsT : forall g, lpreds [::(predT : pred gType)] g = true.
-Proof. ul. elim;rewrite /=; try done;intros. Qed.
+Lemma lpredsT (A : eqType) : forall g, lpreds [::(predT : pred A)] g = true.
+Proof. ul. intros. by simpl. Qed.
 
-Instance traverse_predTG g : {goal lpreds [::predT : pred gType] g}.
+Instance traverse_predTG (A : eqType)  g : {goal lpreds [::predT : pred A] g}.
 constructor. rewrite lpredsT. done. Defined. 
 
-Instance traverse_predTallG (gs : seq gType) : {goal all predT gs}.
+Instance traverse_predTallG  (A : eqType)  (gs : seq A) : {goal all predT gs}.
 constructor. apply/allP=>k. done. Defined. 
 
 Instance goallpreds_allnil (A : eqType) (gs : seq A) : {goal all (lpreds nil) gs}. constructor. unlock lpreds. simpl. induction gs. done. simpl. done. Qed. 
@@ -291,12 +288,51 @@ Instance gType_existsH : {hint exists _ : gType_EqType, True}.
 constructor. exists GEnd.  done. Qed.
 Check lpreds.
 
-Instance hint_size_eq2 (gs gs' : seq gType) x0 : {hint size gs = size gs'} -> {goal x0 < size gs'} -> {goal x0 < size gs}.
+Instance hint_size_eq2  (A : eqType)  (gs gs' : seq A) x0 : {hint size gs = size gs'} -> {goal x0 < size gs'} -> {goal x0 < size gs}.
 Proof. case. move => H. case. move => H0. constructor. rewrite H. done. Qed.
 
+(*Definition in_prede p g  := p \in efv g.
+Notation iprede := in_pred.
 
-Definition in_pred p g  := p \in fv_g g.
-Notation ipred := in_pred.
+Instance ipred_CGPred p : CGPred (ipred p). constructor. constructor. Qed.*)
 
-Instance ipred_CGPred p : CGPred (ipred p). constructor. constructor. Qed.
+(*Important for membership to work*)
+Hint Resolve mem_nth : typeclass_instances.
+
+Instance step_action : forall g l g', {goal step g l g'} -> {goal lpreds [::apred;spred] g} -> {goal apred g'}.  
+Proof.
+move => g l g' [] H [] H0. constructor. elim : H H0; rewrite /=;split_and;cc.
+apply H0. cc.
+apply H0. cc.
+Qed.
+
+Instance step_size : forall g l g',{goal step g l g'} -> {goal lpreds [::apred;spred] g} -> {goal spred g'}.  
+Proof.
+move => g l g' [] H [] H0. constructor.  elim : H H0; rewrite /=;intros;split_and;cc.
+apply H0. cc. rewrite -H.  cc. apply H0. cc. 
+Qed.
+
+
+Instance linear_sgmsg : forall a u g0, {hint Linear (GMsg a u g0)} -> {goal Linear g0}.
+Proof. 
+move => a u g0. apply chint_imp. rewrite /Linear /=.  intros. move : (H (a::aa_p) a0 aa a1). rewrite cat_cons /=. 
+  destruct ( aa_p ++ a0 :: rcons aa a1) eqn:Heqn. case : aa_p H0 Heqn.  done. done.
+  intros. have : Tr ((a::aa_p ++ (a0::aa) ++ [::a1])) (GMsg a u g0). auto.  move/H2 => H3.  move : (H3 H1). 
+  move => [] mi [] mo. intros. auto. 
+Qed.
+
+Instance linear_branch_aux : forall a gs, {hint Linear (GBranch a gs)} -> {goal Forall Linear gs}.  
+Proof.
+move => a gs. apply chint_imp. intros. apply/List.Forall_forall. intros. rewrite /Linear. intros. unfold Linear in H. have : Tr (a::aa_p ++ a0::aa ++ ([::a1])) (GBranch a gs). move : H0.  move/In_in. move/nthP=>Hnth. specialize Hnth with GEnd. destruct Hnth. rewrite -H3 in H1. apply : TRBranch. eauto. apply : H1. 
+intros. apply : H. rewrite -cat_cons in x0. apply : x0. done. 
+Qed.
+
+Instance linear_branch : forall a gs n, {hint Linear (GBranch a gs)} -> {goal n < size gs} -> {goal Linear (nth GEnd gs n)}.
+Proof. intros. destruct H,H0.  apply Build_CHint in H. apply linear_branch_aux in H. destruct H. move : H. move/Forall_forall. intros. constructor. eauto. cc. Qed.
+
+
+Instance linear_unf : forall g n, {hint Linear (GRec n g)} -> {goal Linear g[s GRec n g//n]}.
+Proof. move => g n. apply chint_imp.
+intros.  unfold Linear in *. intros. apply : H. constructor. eauto. done. 
+Qed.
 
