theories/Substitutions.v
@@ -1,56 +1,344 @@
-From mathcomp Require Import all_ssreflect zify.
+From mathcomp Require Import all_ssreflect zify finmap.
 
 Set Implicit Arguments.
 Unset Strict Implicit.
 Unset Printing Implicit Defensive.
-From Dep Require Import Global_Syntax Inductive_Linearity.
-From mathcomp Require Import finmap.
-Let inE := Global_Syntax.inE.
+From Dep Require Import Global_Syntax Utils.
 Open Scope fset_scope.
 Open Scope fmap_scope.
 
+Coercion ptcps_of_act (a : action) := ptcp_from a |` [fset ptcp_to a].
 
-Lemma n_fset0 (n : nat) : [fset n] == fset0 = false.
-Proof. destruct (  ([fset n] == fset0)) eqn:Heqn.  move : Heqn. move/eqP/fsetP=>H. have : n \in [fset n] = false. by rewrite H !inE. 
-rewrite !inE.  done. done.
+Definition label := (action * (value + nat))%type.
+
+Coercion to_action (l : label) : action := l.1.
+
+
+Canonical action_predType := PredType (fun a p => p \in ptcps_of_act a). 
+
+Lemma ptcps_of_act_eq : forall a, ptcps_of_act a = [fset ptcp_from a; ptcp_to a].
+Proof. done. Qed.
+
+Lemma in_action_eq : forall p a, p \in ptcps_of_act a = (p == ptcp_from a) ||  (p == ptcp_to a).
+Proof. intros. destruct a. by rewrite /= /ptcps_of_act !inE /=.  Qed.
+
+Let inE := (inE,ptcps_of_act_eq,Bool.negb_involutive,eqxx,negb_or,negb_and).
+Definition env := {fmap ptcp -> endpoint}.  
+Definition fset_ptcp := {fset ptcp}.
+
+Module Substitution.
+
+Definition axiom_nop (T : eqType) (substitute : nat -> T -> T ->T) (fv : T -> {fset nat})  :=  forall t t0 i, i \notin fv t -> substitute i t t0 = t.
+
+Definition axiom_fv_subst (T : eqType) (substitute : nat -> T -> T ->T) (fv : T -> {fset nat}) :=  
+forall t t0 i, fv t0 = fset0 -> fv (substitute i t t0) = fv t `\ i . 
+
+Record mixin_of (T : eqType) := Mixin {substitute : nat -> T -> T -> T; fv : T -> {fset nat};
+                                                        _ : axiom_nop substitute fv;
+                                                        _ : axiom_fv_subst substitute fv;}.
+Notation class_of := mixin_of.
+
+Record type : Type := Pack {sort : eqType; class : class_of sort; }.
+End Substitution. 
+Coercion Substitution.sort : Substitution.type >-> Equality.type.
+
+Notation substType := Substitution.type.
+Definition substitute T := Substitution.substitute (Substitution.class T).
+Definition fv T := Substitution.fv (Substitution.class T).
+Definition bound (A : substType) (g  : A)  :=  fv g == fset0.
+Arguments bound {_}.
+Print Substitution.sort.
+Arguments substitute {_} _ _ _ : simpl never.
+Arguments fv {_} _ : simpl never.
+
+Notation "G [s G0 // X ]" :=  (substitute X G G0)(at level 0, format "G [s  G0  //  X ]").
+
+Lemma subst_nop ( A: substType) : Substitution.axiom_nop (@substitute A) (@fv A). 
+Proof.  destruct A. destruct class. done. Qed.
+
+Lemma fv_subst ( A: substType) : Substitution.axiom_fv_subst (@substitute A) (@fv A). 
+Proof.  destruct A. destruct class. done. Qed.
+
+Fixpoint gType_substitution (i : nat) g0 g1  :=
+match g0 with
+| GMsg a u g0' => GMsg a u (gType_substitution i g0' g1)
+| GBranch a gs => GBranch a (map (fun g0' => gType_substitution i g0' g1) gs)
+| GVar n => if n == i then g1 else g0
+| GRec n g0' => if n == i then g0 else GRec n (gType_substitution i g0' g1)
+| GEnd => GEnd
+end.
+
+Fixpoint gType_fv (g : gType) :=
+match g with
+| GVar j => [fset j]
+| GEnd => fset0
+| GMsg _ _ g0 => gType_fv g0
+| GBranch _ gs => \bigcup_( i <- map gType_fv gs) i 
+| GRec n g0 => (gType_fv g0) `\ n
+end.
+
+Fixpoint ptcps (g : gType) : {fset ptcp} := 
+match g with 
+| GMsg a _ g0 => a `|`(ptcps g0)
+| GBranch a gs => a `|` \bigcup_( i <- map ptcps gs) i
+| GRec n g0 => ptcps g0
+| _ => fset0
+end.
+
+Canonical gType_predType := PredType (fun g p => p \in ptcps g). 
+
+
+
+Lemma gType_axiom_nop : Substitution.axiom_nop gType_substitution gType_fv.
+Proof. elim;rewrite /=;try done;intros. move : H. rewrite !inE.  rewrite neg_sym. move/negbTE=>->. done. 
+move : H0. rewrite !inE. move/orP=>[]. intros. by  rewrite eq_sym a. rifliad. intros. f_equal. auto. f_equal. 
+auto.
+f_equal. rewrite big_map in H0.  induction l. done. simpl. f_equal.  apply H.  rewrite !inE.  lia. move : H0. 
+rewrite big_cons. rewrite !inE. split_and. apply IHl. intros. apply H. rewrite !inE H1. lia. done. move : H0.  rewrite big_cons !inE. split_and. 
+Qed.
+
+Lemma big_exists : forall (A : eqType) (B : choiceType) (l : seq A) (f0 : A -> {fset B}) p, p \in \bigcup_(j <- l) (f0 j) = has (fun x => p \in f0 x) l. 
+Proof. 
+move => A B. elim. move => f0 p. rewrite big_nil. done. intros. simpl. rewrite big_cons !inE. destruct ( (p \in f0 a) ) eqn:Heqn;rewrite /=. 
+done.
+apply H.
+Qed.
+
+Lemma big_f_eq : forall (A : eqType) (B : choiceType)  (l : seq A) (f : A -> {fset B}) f1, (forall g, g \in l -> f g = f1 g) ->  \bigcup_(j <- l) (f j) =  \bigcup_(j <- l) (f1 j).
+Proof. move => A B. elim. intros. by rewrite !big_nil.
+intros. rewrite !big_cons. f_equal. auto. apply H. auto. 
+Qed.
+
+Lemma big_if : forall (A : eqType) (B : choiceType) (l : seq A) (p : pred A) (f : A -> {fset B}) S, 
+                  \bigcup_(j <- l) (if p j then f j `|` S else f j) = 
+                   (\bigcup_(j <- l) (f j)) `|` (if has p l then S else fset0).
+Proof. move => A B. elim. intros. rewrite !big_nil /=. apply/fsetP=>k. by rewrite !inE. 
+intros. rewrite !big_cons /= H. rifliad. all : apply/fsetP=>k; rewrite !inE; lia. 
+Qed.
+
+Lemma big_cup_in : forall (A : eqType) (B: choiceType) n (l : seq A) (f0 f1 : A -> {fset B}), (forall x n, x \in l -> n \in (f0 x) -> n \in (f1 x)) -> n \in \bigcup_(j <- l) (f0 j) ->  n \in \bigcup_(j <- l) (f1 j).
+Proof. move => A B n. elim. move => f0 f1.  rewrite big_nil. done. intros. move : H1. rewrite !big_cons !inE. move/orP=>[].  intros. rewrite H0 //=. intros. erewrite H. lia. intros. apply H0. eauto. eauto. apply b. 
 Qed.
 
 
-Ltac split_and := intros;repeat (match goal with 
-                   | [ H : is_true (_ && _) |- _ ] => destruct (andP H);clear H
-                   | [ |- is_true (_ && _) ] => apply/andP;split 
 
-                  end);auto.
+Lemma gType_axiom_fv_subst : Substitution.axiom_fv_subst gType_substitution gType_fv.
+Proof. 
+elim;rewrite /=;intros;apply/fsetP=>k;rewrite !inE.
+- rifliad. rewrite (eqP H0). move : H.  move=>->. rewrite !inE. lia. 
+- rewrite /= !inE. destruct (eqVneq k n). subst. lia. lia. 
+- lia.
+- rifliad. rewrite /= (eqP H1) !inE. destruct (k != i);rewrite /=. done. done.
+- rewrite /= H //= !inE. destruct (k != n);rewrite /=;try lia.  rewrite H //= !inE. done.
+- rewrite !big_map. induction l. rewrite !big_nil !inE. lia. 
+  rewrite !big_cons !inE H //= !inE. destruct (k != i);rewrite /=. destruct (k \in gType_fv a0) eqn:Heqn; rewrite Heqn //=.
+  rewrite /= in IHl. apply IHl. intros. apply H. eauto. done. rewrite /= in IHl. apply IHl. intros. apply H. eauto. done.
+Qed.
 
-Lemma mu_height_subst : forall g0 g1  i, guarded i g0 -> contractive g0 -> mu_height (g0[g g1//i]) = mu_height g0.
+Definition gType_substMixin := Substitution.Mixin  gType_axiom_nop gType_axiom_fv_subst.
+Canonical gType_substType := @Substitution.Pack _ gType_substMixin.
+
+
+
+
+
+Ltac fsetPtac := let k := fresh "k" in apply/fsetP=>k;rewrite ?inE;try lia.
+
+(*Definition axiom_ptcps_subst T (substitute : nat -> T -> T ->T) (fv : T -> {fset nat}) (ptcps : T -> fset_ptcp)  :=  
+*)
+
+
+
+
+Fixpoint endpoint_substitution (i : nat) g0 g1  :=
+match g0 with
+| EMsg d a u g0' => EMsg d a u (endpoint_substitution i g0' g1)
+| EBranch d a gs => EBranch d a (map (fun g0' => endpoint_substitution i g0' g1) gs)
+| EVar n => if n == i then g1 else g0
+| ERec n g0' => if n == i then g0 else ERec n (endpoint_substitution i g0' g1)
+| EEnd => EEnd
+end.
+
+Fixpoint endpoint_fv (g : endpoint) :=
+match g with
+| EVar j => [fset j]
+| EEnd => fset0
+| EMsg _ _ _ g0 => endpoint_fv g0
+| EBranch _ _ gs => \bigcup_( i <- map endpoint_fv gs) i 
+| ERec n g0 => (endpoint_fv g0) `\ n
+end.
+
+Lemma endpoint_axiom_nop : Substitution.axiom_nop endpoint_substitution endpoint_fv.
+Proof. elim;rewrite /=;try done;intros. move : H. rewrite !inE.  rewrite neg_sym. move/negbTE=>->. done. 
+move : H0. rewrite !inE. move/orP=>[]. intros. by  rewrite eq_sym a. rifliad. intros. f_equal. auto. f_equal. 
+auto.
+f_equal. rewrite big_map in H0.  induction l. done. simpl. f_equal.  apply H.  rewrite !inE.  lia. move : H0. 
+rewrite big_cons. rewrite !inE. split_and. apply IHl. intros. apply H. rewrite !inE H1. lia. done. move : H0.  rewrite big_cons !inE. split_and. 
+Qed.
+
+
+Lemma endpoint_axiom_fv_subst : Substitution.axiom_fv_subst endpoint_substitution endpoint_fv.
+Proof. 
+elim;rewrite /=;intros;apply/fsetP=>k;rewrite !inE.
+- rifliad. rewrite (eqP H0). move : H.  move=>->. rewrite !inE. lia. 
+- rewrite /= !inE. destruct (eqVneq k n). subst. lia. lia. 
+- lia.
+- rifliad. rewrite /= (eqP H1) !inE. destruct (k != i);rewrite /=. done. done.
+- rewrite /= H //= !inE. destruct (k != n);rewrite /=;try lia.  rewrite H //= !inE. done.
+- rewrite !big_map. induction l. rewrite !big_nil !inE. lia. 
+  rewrite !big_cons !inE H //= !inE. destruct (k != i);rewrite /=. destruct (k \in endpoint_fv a) eqn:Heqn; rewrite Heqn //=.
+  rewrite /= in IHl. apply IHl. intros. apply H. eauto. done. rewrite /= in IHl. apply IHl. intros. apply H. eauto. done.
+Qed.
+
+Definition endpoint_substMixin := Substitution.Mixin  endpoint_axiom_nop endpoint_axiom_fv_subst.
+Canonical endpoint_substType := @Substitution.Pack _ endpoint_substMixin.
+
+
+
+Lemma gType_substitute_substitute : gType_substitution = substitute.  
+Proof. done. Qed.
+
+Lemma gType_fv_fv :  gType_fv = fv. done. Qed.
+
+Lemma substitute_gType_substitute : substitute = gType_substitution.
+Proof. done. Qed.
+
+Lemma fv_gType_fv :  fv = gType_fv.
+Proof. done. Qed.
+
+Lemma endpoint_substitute_substitute : endpoint_substitution = substitute.  
+Proof. done. Qed.
+
+Lemma endpoint_fv_fv :  endpoint_fv = fv. done. Qed.
+
+Lemma substitute_endpoint_substitute : substitute = endpoint_substitution.
+Proof. done. Qed.
+
+Lemma fv_endpoint_fv :  fv = endpoint_fv.
+Proof. done. Qed.
+
+Let unf := (substitute_gType_substitute,fv_gType_fv, substitute_endpoint_substitute,fv_endpoint_fv).
+Let fold := (gType_substitute_substitute,gType_fv_fv,endpoint_substitute_substitute,endpoint_fv_fv).
+Ltac rs :=  rewrite ?unf /= ?fold.
+Ltac rs_in H :=  rewrite ?unf /= ?fold in H.
+
+
+Lemma ptcps_subst : forall t t0 i, ptcps (t[s t0//i]) = if i \in fv t then ptcps t `|` ptcps t0  else ptcps t. 
+Proof. elim;rewrite /=;intros; rewrite /=.
+- rifliad. apply/fsetP=>k;rewrite !inE. rewrite /=. rewrite unf in H.  rs. rs_in H. rewrite !inE in H. by rewrite eq_sym H. rs. 
+  rs_in H. rewrite !inE in H.  rewrite eq_sym H. by simpl. done. rs. rewrite /=. fsetPtac. rifliad. split_and. lia. 
+  split_and. rs.  rewrite !inE H H3 !inE. done. rs. rewrite H. move : H1.  move/andP/andP. rewrite !inE. move/orP=>[].  lia. 
+  move/negbTE=>->. done. 
+- rs. rewrite H.   rifliad. fsetPtac. 
+- rs. rewrite !big_map.
+  have :  forall g, g \in l -> ptcps (gType_substitution i g t0) = (if i \in gType_fv g then ptcps g `|` ptcps t0 else ptcps g). auto. move=>HH.
+
+  rewrite (big_f_eq HH) big_if !inE -big_exists. 
+
+  rifliad. rewrite fsetUA. done. rewrite fsetUA. fsetPtac. 
+Qed.
+
+
+
+(*Class SubstType  (A : eqType) := { substitute : nat -> A -> A -> A }.
+
+Instance substtype_gType : SubstType gType_EqType := Build_SubstType substitution.   
+
+Instance substtype_endpoint : SubstType endpoint_EqType := Build_SubstType subst_e.   
+
+
+Notation "G [g G0 // X ]" :=  (substitution X G G0)(at level 0, format "G [g  G0  //  X ]").
+
+Notation "G [e G0 // X ]" :=  (subst_e X G G0)(at level 0, format "G [e  G0  //  X ]").*)
+
+
+
+
+
+(*Fixpoint endpoint_substitution (i : nat) e0 e1  :=
+match e0 with
+| EMsg d a u e0' => EMsg d a u (endpoint_substitution i e0' e1)
+| EBranch d a es => EBranch d a (map (fun e0' => endpoint_substitution i e0' e1) es)
+| EVar n => if n == i then e1 else e0
+| ERec n e0' => if n == i then e0 else ERec n (endpoint_substitution i e0' e1) (*Key insight, consume mu during traversal to make it commute with congruence rules*)
+| EEnd => EEnd
+end.*)
+
+
+(*Fixpoint guarded n g := 
+match g with 
+| GVar n0 => n0 != n
+| GRec n0 g0 => (n == n0) || guarded n g0
+| _ => true
+end.
+
+Fixpoint contractive g := 
+match g with 
+| GRec n g0 => (guarded n g0) && (contractive g0)
+| GMsg a u g0 => contractive g0
+| GBranch a gs => all contractive gs 
+| _ => true 
+end.*)
+
+
+(*Fixpoint mu_height g :=
+match g with
+| GRec n g0 => (mu_height g0).+1
+| _ => 0
+end.*)
+
+(*Definition unf g := if g is GRec n g' then (substitution n g' g) else g.
+
+Open Scope fset_scope.
+Open Scope fmap_scope.*)
+
+
+
+
+ 
+
+(*Lemma in_ptcp_of_act_f : forall a, (ptcp_from a \in a).
+Proof. case. intros. rewrite //=. by  rewrite /ptcps_of_act //= !inE eqxx. Qed.
+
+Lemma in_ptcp_of_act_t : forall a, (ptcp_to a \in ptcps_of_act a).
+Proof. case. intros. rewrite //=.  rewrite /ptcps_of_act //= !inE eqxx. lia. Qed.
+*)
+
+
+
+
+
+
+
+
+
+
+
+(*Notation negb_invol :=  Bool.negb_involutive.*)
+
+
+
+
+
+
+(*Lemma n_fset0 (n : nat) : [fset n] == fset0 = false.
+Proof. destruct (  ([fset n] == fset0)) eqn:Heqn.  move : Heqn. move/eqP/fsetP=>H. have : n \in [fset n] = false. by rewrite H !inE. 
+rewrite !inE.  done. done.
+Qed.*)
+
+
+(*Lemma mu_height_subst : forall g0 g1  i, guarded i g0 -> contractive g0 -> mu_height (g0[g g1//i]) = mu_height g0.
 Proof. 
 elim; try solve [by rewrite /=].
 - rewrite /=. intros. split_and. rewrite (negbTE H). done. 
 - intros. simpl. simpl in H0. split_and. destruct (i == n) eqn:Heqn.  rewrite eq_sym Heqn. done.  
   simpl in H1. rifliad. split_and. simpl. f_equal. apply H.  done. done. 
-Qed.
-Lemma my_in_cons : forall (A :eqType) (a : A) l, a \in (a::l).
-Proof. intros. rewrite !inE. done. Qed.
-
-Lemma my_in_cons2 : forall (A :eqType) (a a0 : A) l, a \in l -> a \in (a0::l).
-Proof. intros. rewrite !inE H. lia. Qed.
-
-Hint Resolve my_in_cons my_in_cons2.
-Lemma fv_g_subst : forall g g0 n, bound g0 -> fv_g (g[g g0 // n]) = fv_g g `\ n. 
-Proof. 
-elim;rewrite /=;intros;apply/fsetP=>k;rewrite !inE.
-- rifliad. rewrite (eqP H0). move : H.  rewrite /bound. move/eqP=>->. rewrite !inE. by destruct (eqVneq k n0).
-- rewrite /= !inE. destruct (eqVneq k n). subst. lia. lia. 
-- lia.
-- rifliad. rewrite /= (eqP H1) !inE. destruct (k != n0);rewrite /=. done. done.
-- rewrite /= H //= !inE. destruct (k != n);rewrite /=;try lia.  rewrite H //= !inE. done.
-- rewrite !big_map. induction l. rewrite !big_nil !inE. lia. 
-  rewrite !big_cons !inE H //= !inE. destruct (k != n);rewrite /=. destruct (k \in fv_g a0) eqn:Heqn;rewrite Heqn //=.
-  rewrite /= in IHl. apply IHl. intros. apply H. eauto. done. rewrite /= in IHl. apply IHl. intros. apply H. eauto. done.
-Qed.
+Qed.*)
 
 
-Lemma bound_subst : forall (g g': gType) i, fv_g g = [fset i] -> bound g' -> bound (substitution i g g').
+
+
+(*Lemma bound_subst : forall (g g': gType) i, fv_g g = [fset i] -> bound g' -> bound (substitution i g g').
 Proof. intros. move : H0. rewrite /bound. move/eqP=>HH. rewrite -HH. apply/eqP.  rewrite fv_g_subst. rewrite H HH. apply/fsetP=>k. rewrite !inE. destruct (eqVneq k i);done.  rewrite /bound. by apply/eqP.
 Qed.
 
@@ -67,21 +355,14 @@ Proof. intros. apply notin_guarded. apply bound_notin. done. Qed.
 Lemma guarded_subst : forall g g' n i, guarded n g -> bound g' -> guarded n (g)[g g' // i].
 Proof. elim;rewrite /=;intros. rifliad. apply bound_guarded. done. all:auto. 
 rifliad. simpl. destruct (orP H0). by rewrite H3.  rewrite H //=. lia.
-Qed.
+Qed.*)
 
 
-Lemma big_cup_in : forall (A : eqType) (B: choiceType) n (l : seq A) (f0 f1 : A -> {fset B}), (forall x n, x \in l -> n \in (f0 x) -> n \in (f1 x)) -> n \in \bigcup_(j <- l) (f0 j) ->  n \in \bigcup_(j <- l) (f1 j).
-Proof. move => A B n. elim. move => f0 f1.  rewrite big_nil. done. intros. move : H1. rewrite !big_cons !inE. move/orP=>[].  intros. rewrite H0 //=. intros. erewrite H. lia. intros. apply H0. eauto. eauto. apply b. 
-Qed.
 
-Lemma foldr_exists : forall (A : eqType) (B : choiceType) (l : seq A) (f0 : A -> {fset B}) p, p \in \bigcup_(j <- l) (f0 j) = has (fun x => p \in f0 x) l. 
-Proof. 
-move => A B. elim. move => f0 p. rewrite big_nil. done. intros. simpl. rewrite big_cons !inE. destruct ( (p \in f0 a) ) eqn:Heqn;rewrite /=. 
-done.
-apply H.
-Qed.
 
-Lemma contractive_subst : forall (g g': gType) i, (*i \in fv_g g ->*) contractive g -> contractive g' -> bound g' -> contractive (substitution i g g').
+
+
+(*Lemma contractive_subst : forall (g g': gType) i, (*i \in fv_g g ->*) contractive g -> contractive g' -> bound g' -> contractive (substitution i g g').
 Proof.
 elim;  (try solve [rewrite /= ;auto]).
 - rewrite/=. move => v g' i j. case : (eqVneq v i).  done. simpl. done.
@@ -98,24 +379,8 @@ Qed.
 
 Notation gt_pred g := (bound g && contractive g). 
 
-Lemma neg_sym : forall (A : eqType) (a b : A), (a != b) = (b != a).
-Proof.
-intros. destruct (eqVneq a b).  done. done. 
-Qed.
 
 
-
-Notation negb_invol :=  Bool.negb_involutive.
-
-
-Lemma subst_nop : forall g g' x, x \notin (fv_g g) -> substitution x g g' = g. 
-Proof. 
-elim;rewrite /=;try done;intros. move : H. rewrite !inE.  rewrite neg_sym. move/negbTE=>->. done. 
-move : H0. rewrite !inE. move/orP=>[]. intros. by  rewrite eq_sym a. rifliad. intros. f_equal. auto. f_equal. 
-auto.
-f_equal. rewrite big_map in H0.  induction l. done. simpl. f_equal.  apply H.  rewrite !inE.  lia. move : H0. 
-rewrite big_cons. rewrite !inE. split_and. apply IHl. intros. apply H. rewrite !inE H1. lia. done. move : H0.  rewrite big_cons !inE. split_and. 
-Qed.
 
 Lemma unf_pred : forall (g : gType), gt_pred  g -> gt_pred (unf g).
 Proof.
@@ -154,13 +419,13 @@ intros. simpl in *. apply (mu_height_iter_unf k) in H. move : H.
 have : mu_height sg - k  = 0 by lia. move=>->. intros. destruct ((iter k (fun g => unf g) sg));try done.
 Qed.
 
-Notation full_unf g := (iter (mu_height g) (fun g' => unf g') g).
+Notation full_unf g := (iter (mu_height g) (fun g' => unf g') g).*)
 
 
 (*Endpoint type*)
 
 
-Fixpoint eguarded n g := 
+(*Fixpoint eguarded n g := 
 match g with 
 | EVar n0 => n0 != n
 | ERec n0 g0 => (n == n0) || eguarded n g0
@@ -173,18 +438,11 @@ match g with
 | EMsg _ a u g0 => econtractive g0
 | EBranch _ a gs => all econtractive gs 
 | _ => true 
-end.
+end.*)
 
-Fixpoint efv g  :=
-  match g with
-  | EVar j => [fset j]
-  | EEnd => fset0
-  | EMsg _ _ _ g0 => efv g0
-  | EBranch _ _ gs => \bigcup_( i <- map efv gs) i 
-  | ERec n g0 => (efv g0) `\ n
-  end.
 
-Definition ebound g := efv g == fset0.
+
+(*Definition ebound g := efv g == fset0.
 
 
 Fixpoint emu_height g :=
@@ -208,7 +466,7 @@ Qed.
 Lemma fsubset_in : forall (A : choiceType) (b c : {fset A}), b `<=` c -> (forall j, j \in b -> j \in c).
 Proof.
 intros. Search _ fsub1set. move : H0. rewrite -!fsub1set.  intros. apply : fsubset_trans. apply : H0. apply H. 
-Qed.
+Qed.*)
 
 (*Lemma efv_subst : forall g g0 n, efv g0 `<=` efv g  -> efv (g[e g0 // n]) = efv g `\ n. 
 Proof. 
@@ -224,7 +482,7 @@ destruct (k \in efv g0). destruct (eqVneq k n). specialize HH with k. rewrite -H
   rewrite /= in IHl. apply IHl. intros. apply H. eauto. done. rewrite /= in IHl. apply IHl. intros. apply H. eauto. done.
 Qed.*)
 
-Lemma efv_subst : forall g g0 n, ebound g0 -> efv (g[e g0 // n]) = efv g `\ n. 
+(*Lemma efv_subst : forall g g0 n, ebound g0 -> efv (g[e g0 // n]) = efv g `\ n. 
 Proof. 
 elim;rewrite /=;intros;apply/fsetP=>k;rewrite !inE.
 - rifliad. rewrite (eqP H0). move : H.  rewrite /bound. move/eqP=>->. rewrite !inE. by destruct (eqVneq k n0).
@@ -383,3 +641,4 @@ elim;rewrite /=;intros;apply/fsetP=>k;rewrite !inE.
   rewrite /= in IHl. apply IHl. intros. apply H. eauto.  done. rewrite /= in IHl. apply IHl. intros. apply H. eauto. done.
 Qed.
 
+*)
